access: Tcb_AC arch split
Signed-off-by: Ryan Barry <ryan.barry@unsw.edu.au>

proof/access-control/Tcb_AC.thy
@@ -5,39 +5,34 @@
  *)
 
 theory Tcb_AC
-imports Finalise_AC
+imports ArchFinalise_AC
 begin
-
-context begin interpretation Arch . (*FIXME: arch_split*)
 
 (* FIXME-NTFN: The 'NotificationControl' case of the following definition needs to be changed. *)
 
-definition
-  authorised_tcb_inv :: "'a PAS \<Rightarrow> Invocations_A.tcb_invocation \<Rightarrow>  bool"
-where
+definition authorised_tcb_inv :: "'a PAS \<Rightarrow> tcb_invocation \<Rightarrow>  bool" where
  "authorised_tcb_inv aag ti \<equiv> case ti of
-     tcb_invocation.Suspend t \<Rightarrow> is_subject aag t
-   | tcb_invocation.Resume t \<Rightarrow> is_subject aag t
-   | tcb_invocation.ThreadControl t sl ep mcp priority croot vroot buf
-          \<Rightarrow> is_subject aag t \<and>
-            (\<forall>(cap, slot) \<in> (set_option croot \<union> set_option vroot \<union>
-                            (case_option {} (set_option \<circ> snd) buf)).
-                      pas_cap_cur_auth aag cap \<and> is_subject aag (fst slot))
-   | tcb_invocation.NotificationControl t ntfn \<Rightarrow> is_subject aag t \<and>
-         case_option True (\<lambda>a. \<forall>auth \<in> {Receive, Reset}.
-                                 (pasSubject aag, auth, pasObjectAbs aag a) \<in> pasPolicy aag) ntfn
-   | tcb_invocation.ReadRegisters src susp n arch \<Rightarrow> is_subject aag src
-   | tcb_invocation.WriteRegisters dest res values arch \<Rightarrow> is_subject aag dest
-   | tcb_invocation.CopyRegisters dest src susp res frame int_regs arch \<Rightarrow>
-         is_subject aag src \<and> is_subject aag dest
-   | tcb_invocation.SetTLSBase tcb tls_base \<Rightarrow> is_subject aag tcb"
+    Suspend t \<Rightarrow> is_subject aag t
+  | Resume t \<Rightarrow> is_subject aag t
+  | ThreadControl t sl ep mcp priority croot vroot buf \<Rightarrow>
+      is_subject aag t \<and>
+      (\<forall>(cap, slot) \<in> set_option croot \<union> set_option vroot \<union>
+                      (case_option {} (set_option \<circ> snd) buf). pas_cap_cur_auth aag cap \<and>
+                                                               is_subject aag (fst slot))
+  | NotificationControl t ntfn \<Rightarrow>
+      is_subject aag t \<and>
+      case_option True (\<lambda>a. \<forall>auth \<in> {Receive, Reset}. aag_has_auth_to aag auth a) ntfn
+  | ReadRegisters src susp n arch \<Rightarrow> is_subject aag src
+  | WriteRegisters dest res values arch \<Rightarrow> is_subject aag dest
+  | CopyRegisters dest src susp res frame int_regs arch \<Rightarrow> is_subject aag src \<and> is_subject aag dest
+  | SetTLSBase tcb tls_base \<Rightarrow> is_subject aag tcb"
 
 subsection\<open>invoke\<close>
 
 lemma setup_reply_master_respects:
   "\<lbrace>integrity aag X st and K (is_subject aag t)\<rbrace>
-     setup_reply_master t
-   \<lbrace>\<lambda>rv. integrity aag X st\<rbrace>"
+   setup_reply_master t
+   \<lbrace>\<lambda>_. integrity aag X st\<rbrace>"
   apply (simp add: setup_reply_master_def)
   apply (wp get_cap_wp set_cap_integrity_autarch[unfolded K_def pred_conj_def]
             set_original_integrity_autarch)+
@@ -48,96 +43,70 @@ crunch eintegrity[wp]: possible_switch_to "integrity aag X st"
   (ignore: tcb_sched_action)
 
 lemma restart_integrity_autarch:
-  "\<lbrace>integrity aag X st and K (is_subject aag t) and einvs
-           and tcb_at t
-           and pas_refined aag\<rbrace>
-     restart t
-   \<lbrace>\<lambda>rv. integrity aag X st\<rbrace>"
+  "\<lbrace>integrity aag X st and K (is_subject aag t) and einvs and tcb_at t and pas_refined aag\<rbrace>
+   restart t
+   \<lbrace>\<lambda>_. integrity aag X st\<rbrace>"
   apply (simp add: restart_def)
   apply (wp set_thread_state_integrity_autarch setup_reply_master_respects
             hoare_drop_imps
-        | simp add: if_apply_def2)+
+         | simp add: if_apply_def2)+
   done
 
 crunch integrity_autarch: option_update_thread "integrity aag X st"
 
 crunch arch_state [wp]: cap_swap_for_delete "\<lambda>s. P (arch_state s)"
 
-lemma schematic_lift_tuple3_l:
-  "P (fst (a, b, c)) (fst (snd (a, b, c))) (snd (snd (a, b, c))) \<and> Q \<Longrightarrow> P a b c" by simp
-
-lemma schematic_lift_tuple3_r:
-  "Q \<and> P (fst (a, b, c)) (fst (snd (a, b, c))) (snd (snd (a, b, c))) \<Longrightarrow> P a b c" by simp
-
-(* FIXME: MOVE *)
-lemma invoke_tcb_cases:
-  "invoke_tcb ti = (case ti of
-     tcb_invocation.Suspend t \<Rightarrow> invoke_tcb (tcb_invocation.Suspend t)
-   | tcb_invocation.Resume t \<Rightarrow> invoke_tcb (tcb_invocation.Resume t)
-   | tcb_invocation.ThreadControl t sl ep mcp priority croot vroot buf \<Rightarrow>
-         invoke_tcb (tcb_invocation.ThreadControl t sl ep mcp priority croot vroot buf)
-   | tcb_invocation.NotificationControl t ntfn \<Rightarrow>
-         invoke_tcb (tcb_invocation.NotificationControl t ntfn)
-   | tcb_invocation.ReadRegisters src susp n arch \<Rightarrow>
-         invoke_tcb (tcb_invocation.ReadRegisters src susp n arch)
-   | tcb_invocation.WriteRegisters dest res values arch \<Rightarrow>
-         invoke_tcb (tcb_invocation.WriteRegisters dest res values arch)
-   | tcb_invocation.CopyRegisters dest src susp res frame int_regs arch \<Rightarrow>
-         invoke_tcb (tcb_invocation.CopyRegisters dest src susp res frame int_regs arch)
-   | tcb_invocation.SetTLSBase tcb tls_base \<Rightarrow> invoke_tcb (tcb_invocation.SetTLSBase tcb tls_base))"
-  by (cases ti, simp_all)
-
-lemmas itr_wps = restart_integrity_autarch as_user_integrity_autarch thread_set_integrity_autarch
-              option_update_thread_integrity_autarch thread_set_pas_refined
-              cap_insert_integrity_autarch cap_insert_pas_refined
-              hoare_vcg_all_liftE hoare_weak_lift_impE hoare_weak_lift_imp hoare_vcg_all_lift
-              check_cap_inv[where P="valid_cap c" for c]
-              check_cap_inv[where P="tcb_cap_valid c p" for c p]
-              check_cap_inv[where P="cte_at p0" for p0]
-              check_cap_inv[where P="tcb_at p0" for p0]
-              check_cap_inv[where P="ex_cte_cap_wp_to P p" for P p]
-              check_cap_inv[where P="ex_nonz_cap_to p" for p]
-              check_cap_inv2[where Q="\<lambda>_. integrity aag X st" for aag X st]
-              check_cap_inv2[where Q="\<lambda>_. pas_refined aag" for aag]
-              checked_insert_no_cap_to cap_insert_ex_cap
-              cap_delete_valid_cap cap_delete_deletes
-              hoare_case_option_wp thread_set_valid_cap
-              thread_set_tcb_ipc_buffer_cap_cleared_invs
-              thread_set_invs_trivial[OF ball_tcb_cap_casesI]
-              thread_set_cte_wp_at_trivial[where Q="\<lambda>x. x", OF ball_tcb_cap_casesI]
-              thread_set_no_cap_to_trivial[OF ball_tcb_cap_casesI]
+lemmas itr_wps =
+  restart_integrity_autarch as_user_integrity_autarch thread_set_integrity_autarch
+  option_update_thread_integrity_autarch thread_set_pas_refined
+  cap_insert_integrity_autarch cap_insert_pas_refined
+  hoare_vcg_all_liftE wp_throw_const_impE hoare_weak_lift_imp hoare_vcg_all_lift
+  check_cap_inv[where P="valid_cap c" for c]
+  check_cap_inv[where P="tcb_cap_valid c p" for c p]
+  check_cap_inv[where P="cte_at p0" for p0]
+  check_cap_inv[where P="tcb_at p0" for p0]
+  check_cap_inv[where P="ex_cte_cap_wp_to P p" for P p]
+  check_cap_inv[where P="ex_nonz_cap_to p" for p]
+  check_cap_inv2[where Q="\<lambda>_. integrity aag X st" for aag X st]
+  check_cap_inv2[where Q="\<lambda>_. pas_refined aag" for aag]
+  checked_insert_no_cap_to cap_insert_ex_cap
+  cap_delete_valid_cap cap_delete_deletes
+  hoare_case_option_wp thread_set_valid_cap
+  thread_set_tcb_ipc_buffer_cap_cleared_invs
+  thread_set_invs_trivial[OF ball_tcb_cap_casesI]
+  thread_set_cte_wp_at_trivial[where Q="\<lambda>x. x", OF ball_tcb_cap_casesI]
+  thread_set_no_cap_to_trivial[OF ball_tcb_cap_casesI]
 
 (*FIXME MOVE *)
-
 lemma aag_cap_auth_master_Reply:
-  "\<lbrakk>pas_refined aag s ; AllowGrant \<in> R\<rbrakk>
-     \<Longrightarrow>  pas_cap_cur_auth aag (cap.ReplyCap tcb True R) = is_subject aag tcb"
+  "\<lbrakk> pas_refined aag s ; AllowGrant \<in> R \<rbrakk>
+     \<Longrightarrow>  pas_cap_cur_auth aag (ReplyCap tcb True R) = is_subject aag tcb"
   unfolding aag_cap_auth_def
   by (fastforce intro: aag_wellformed_refl aag_wellformed_control_is_owns[THEN iffD1]
                  simp: pas_refined_def cli_no_irqs clas_no_asid cap_auth_conferred_def
                        reply_cap_rights_to_auth_def)
 
-
-
 (* FIXME MOVE *)
 lemma cdt_NullCap:
-  "valid_mdb s \<Longrightarrow> caps_of_state s src = Some NullCap \<Longrightarrow> cdt s src = None"
+  "\<lbrakk> valid_mdb s; caps_of_state s src = Some NullCap \<rbrakk>
+     \<Longrightarrow> cdt s src = None"
   by (rule ccontr) (force dest: mdb_cte_atD simp: valid_mdb_def2)
-
 
 lemma setup_reply_master_pas_refined:
   "\<lbrace>pas_refined aag and valid_mdb and K (is_subject aag t)\<rbrace>
-     setup_reply_master t
-   \<lbrace>\<lambda>rv. pas_refined aag\<rbrace>"
+   setup_reply_master t
+   \<lbrace>\<lambda>_. pas_refined aag\<rbrace>"
   apply (simp add: setup_reply_master_def)
   apply (wp get_cap_wp set_cap_pas_refined set_original_wp)+
   by (force dest: cdt_NullCap simp: aag_cap_auth_master_Reply cte_wp_at_caps_of_state)
 
 crunches possible_switch_to
-  for tcb_domain_map_wellformed[wp]: " tcb_domain_map_wellformed aag"
+  for tcb_domain_map_wellformed[wp]: "tcb_domain_map_wellformed aag"
 
 lemma restart_pas_refined:
-  "\<lbrace>pas_refined aag and invs and tcb_at t and K (is_subject aag t)\<rbrace> restart t \<lbrace>\<lambda>rv. pas_refined aag\<rbrace>"
+  "\<lbrace>pas_refined aag and invs and tcb_at t and K (is_subject aag t)\<rbrace>
+   restart t
+   \<lbrace>\<lambda>_. pas_refined aag\<rbrace>"
   apply (simp add: restart_def get_thread_state_def)
   apply (wp set_thread_state_pas_refined setup_reply_master_pas_refined thread_get_wp'
          | strengthen invs_mdb
@@ -149,21 +118,24 @@ lemma option_update_thread_set_safe_lift:
      \<Longrightarrow> \<lbrace>P\<rbrace> option_update_thread t f v \<lbrace>\<lambda>rv. P\<rbrace>"
   by (simp add: option_update_thread_def split: option.split)
 
-lemmas option_update_thread_pas_refined
-    = option_update_thread_set_safe_lift [OF thread_set_pas_refined]
+lemmas option_update_thread_pas_refined =
+  option_update_thread_set_safe_lift [OF thread_set_pas_refined]
 
 crunch integrity_autarch[wp]: thread_set_priority "integrity aag X st"
   (ignore: tcb_sched_action)
 
 lemma set_priority_integrity_autarch[wp]:
  "\<lbrace>integrity aag X st and pas_refined aag and K (is_subject aag tptr)\<rbrace>
-    set_priority tptr prio \<lbrace>\<lambda>_. integrity aag X st\<rbrace>"
+  set_priority tptr prio
+  \<lbrace>\<lambda>_. integrity aag X st\<rbrace>"
   by (simp add: set_priority_def | wp)+
 
 lemma set_priority_pas_refined[wp]:
   "\<lbrace>pas_refined aag\<rbrace>
-    set_priority tptr prio \<lbrace>\<lambda>_. pas_refined aag\<rbrace>"
-  apply (simp add: set_priority_def thread_set_priority_def ethread_set_def set_eobject_def get_etcb_def
+   set_priority tptr prio
+   \<lbrace>\<lambda>_. pas_refined aag\<rbrace>"
+  apply (simp add: set_priority_def thread_set_priority_def
+                   ethread_set_def set_eobject_def get_etcb_def
          | wp hoare_vcg_imp_lift')+
    apply (simp add: tcb_sched_action_def | wp)+
   apply (clarsimp simp: etcb_at_def pas_refined_def tcb_domain_map_wellformed_aux_def
@@ -174,7 +146,8 @@ lemma set_priority_pas_refined[wp]:
   apply (force intro: domtcbs split: if_split_asm)
   done
 
-lemma gts_test[wp]: "\<lbrace>\<top>\<rbrace> get_thread_state t \<lbrace>\<lambda>rv s. test rv = st_tcb_at test t s\<rbrace>"
+lemma gts_test[wp]:
+   "\<lbrace>\<top>\<rbrace> get_thread_state t \<lbrace>\<lambda>rv s. test rv = st_tcb_at test t s\<rbrace>"
   apply (simp add: get_thread_state_def thread_get_def)
   apply wp
   apply (clarsimp simp add: st_tcb_def2)
@@ -182,52 +155,30 @@ lemma gts_test[wp]: "\<lbrace>\<top>\<rbrace> get_thread_state t \<lbrace>\<lamb
 
 crunch exst[wp]: option_update_thread "\<lambda>s. P (exst s)"
 
-lemma out_valid_sched: "(\<And>x a. tcb_state (f a x) = tcb_state x) \<Longrightarrow>
-  \<lbrace>valid_sched\<rbrace> option_update_thread tptr f v \<lbrace>\<lambda>rv. valid_sched\<rbrace>"
-  apply (simp add: option_update_thread_def)
-  apply (rule hoare_pre)
-  apply (wp thread_set_not_state_valid_sched | wpc | simp)+
-  done
-
-
-definition "safe_id x \<equiv> x"
-
-lemma use_safe_id: "safe_id x \<Longrightarrow> x"
-  by (simp add: safe_id_def)
-
-lemma simplify_post:
-  "\<lbrakk>\<And>r s. x r s \<Longrightarrow> safe_id (Q' r s) \<Longrightarrow> Q r s; \<lbrace>P\<rbrace> f \<lbrace>\<lambda>r s. x r s \<and> Q' r s\<rbrace>,\<lbrace>E\<rbrace> \<rbrakk>
-    \<Longrightarrow> \<lbrace>P\<rbrace> f \<lbrace>Q\<rbrace>,\<lbrace>E\<rbrace>"
-  apply (rule hoare_post_impErr)
-  apply assumption
-  apply (clarsimp simp add: safe_id_def)+
-  done
-
-end
-
-lemma (in is_extended') valid_cap_syn[wp]: "I (\<lambda>s. valid_cap_syn s a)" by (rule lift_inv,simp)
-
-lemma (in is_extended') no_cap_to_obj_dr_emp[wp]: "I (no_cap_to_obj_dr_emp a)" by (rule lift_inv,simp)
-
-lemma (in is_extended') cte_wp_at[wp]: "I (cte_wp_at P a)" by (rule lift_inv,simp)
-
 crunch pas_refined[wp]: set_mcpriority "pas_refined aag"
 
 crunch integrity_autarch: set_mcpriority "integrity aag X st"
 
-context begin interpretation Arch . (*FIXME: arch_split*)
+lemma (in is_extended') valid_cap_syn[wp]: "I (\<lambda>s. valid_cap_syn s a)"
+  by (rule lift_inv, simp)
+
+lemma (in is_extended') no_cap_to_obj_dr_emp[wp]: "I (no_cap_to_obj_dr_emp a)"
+  by (rule lift_inv, simp)
+
+lemma (in is_extended') cte_wp_at[wp]: "I (cte_wp_at P a)"
+  by (rule lift_inv, simp)
 
 lemma checked_insert_pas_refined:
   "\<lbrace>pas_refined aag and valid_mdb and
-       K(\<not> is_master_reply_cap new_cap \<and> is_subject aag target \<and>
-       is_subject aag (fst src_slot) \<and> pas_cap_cur_auth aag new_cap)\<rbrace>
-     check_cap_at new_cap src_slot (
-     check_cap_at (ThreadCap target) slot(
-     cap_insert new_cap src_slot (target, ref)))
+    K(\<not> is_master_reply_cap new_cap \<and> is_subject aag target \<and>
+      is_subject aag (fst src_slot) \<and> pas_cap_cur_auth aag new_cap)\<rbrace>
+   check_cap_at new_cap src_slot
+     (check_cap_at (ThreadCap target) slot
+        (cap_insert new_cap src_slot (target, ref)))
    \<lbrace>\<lambda>rv. pas_refined aag\<rbrace>"
   apply (unfold check_cap_at_def)
   apply (wp cap_insert_pas_refined_same_object_as get_cap_wp)
-  by (fastforce simp:cte_wp_at_caps_of_state)
+  by (fastforce simp: cte_wp_at_caps_of_state)
 
 (* FIXME MOVE *)
 lemma update_cdt_wp:
@@ -238,9 +189,7 @@ lemma update_cdt_wp:
 lemma parent_ofD: "m \<Turnstile> src \<leadsto> x \<Longrightarrow> m x = Some src"
   by (simp add: cdt_parent_of_def)
 
-
 crunch tcb_states_of_state[wp]: set_untyped_cap_as_full "\<lambda>s. P (tcb_states_of_state s)"
-
 
 (* FIXME MOVE *)
 lemma map_le_to_rtrancl:
@@ -257,15 +206,15 @@ lemma map_le_to_cca:
   by (rule map_le_to_rtrancl)
 
 lemma cap_insert_cdt_change_allowed[wp]:
-  "\<lbrace> valid_mdb and cdt_change_allowed' aag slot\<rbrace>
-     cap_insert new_cap src_slot dest_slot
-  \<lbrace>\<lambda>_. cdt_change_allowed' aag slot \<rbrace>"
+  "\<lbrace>valid_mdb and cdt_change_allowed' aag slot\<rbrace>
+   cap_insert new_cap src_slot dest_slot
+   \<lbrace>\<lambda>_. cdt_change_allowed' aag slot\<rbrace>"
   apply (rule hoare_pre, unfold cap_insert_def)
    apply (wp add: dxo_wp_weak update_cdt_wp | simp)+
         apply (rule hoare_post_imp[of
         "\<lambda>_. cdt_change_allowed' aag slot and (\<lambda>s. cdt s dest_slot = None)"])
          apply (fastforce elim: map_le_to_cca[rotated] simp:map_le_def dom_def)
-        apply (wps|wp get_cap_wp)+
+        apply (wps | wp get_cap_wp)+
   apply (clarsimp)
   apply (drule valid_mdb_mdb_cte_at)
   apply (subst not_Some_eq[symmetric])
@@ -274,84 +223,12 @@ lemma cap_insert_cdt_change_allowed[wp]:
   apply (simp add:cte_wp_at_caps_of_state)
   done
 
-
-lemma invoke_tcb_tc_respects_aag:
-  "\<lbrace> integrity aag X st and pas_refined aag
-         and einvs and simple_sched_action
-         and tcb_inv_wf (ThreadControl t sl ep mcp priority croot vroot buf)
-         and K (authorised_tcb_inv aag (ThreadControl t sl ep mcp priority croot vroot buf))\<rbrace>
-     invoke_tcb (ThreadControl t sl ep mcp priority croot vroot buf)
-   \<lbrace>\<lambda>rv. integrity aag X st and pas_refined aag\<rbrace>"
-  apply (rule hoare_gen_asm)+
-  apply (subst invoke_tcb.simps)
-  apply (subst set_priority_extended.dxo_eq)
-  apply (rule hoare_vcg_precond_imp)
-   apply (rule_tac P="case ep of Some v \<Rightarrow> length v = word_bits | _ \<Rightarrow> True"
-                 in hoare_gen_asm)
-   apply (simp only: split_def)
-  apply ((simp add: conj_comms del: hoare_True_E_R,
-                  strengthen imp_consequent[where Q="x = None" for x], simp cong: conj_cong)
-        | rule wp_split_const_if wp_split_const_if_R
-                   hoare_vcg_all_lift_R
-                   hoare_vcg_E_elim hoare_vcg_const_imp_lift_R
-                   hoare_vcg_R_conj
-        | wp
-             restart_integrity_autarch set_mcpriority_integrity_autarch
-             as_user_integrity_autarch thread_set_integrity_autarch
-             option_update_thread_integrity_autarch
-             out_valid_sched static_imp_wp
-             cap_insert_integrity_autarch checked_insert_pas_refined
-             cap_delete_respects' cap_delete_pas_refined'
-             check_cap_inv2[where Q="\<lambda>_. integrity aag X st"]
-             as_user_pas_refined restart_pas_refined
-             thread_set_pas_refined
-             option_update_thread_pas_refined
-             out_invs_trivial case_option_wpE cap_delete_deletes
-             cap_delete_valid_cap cap_insert_valid_cap out_cte_at
-             cap_insert_cte_at cap_delete_cte_at out_valid_cap out_tcb_valid
-             hoare_vcg_const_imp_lift_R hoare_vcg_all_lift_R
-             thread_set_tcb_ipc_buffer_cap_cleared_invs
-             thread_set_invs_trivial[OF ball_tcb_cap_casesI]
-             hoare_vcg_all_lift thread_set_valid_cap out_emptyable
-             check_cap_inv[where P="valid_cap c" for c]
-             check_cap_inv[where P="tcb_cap_valid c p" for c p]
-             check_cap_inv[where P="cte_at p0" for p0]
-             check_cap_inv[where P="tcb_at p0" for p0]
-             check_cap_inv[where P="simple_sched_action"]
-             check_cap_inv[where P="valid_list"]
-             check_cap_inv[where P="valid_sched"]
-             thread_set_cte_at
-             thread_set_cte_wp_at_trivial[where Q="\<lambda>x. x", OF ball_tcb_cap_casesI]
-             thread_set_no_cap_to_trivial[OF ball_tcb_cap_casesI]
-             checked_insert_no_cap_to
-             out_no_cap_to_trivial[OF ball_tcb_cap_casesI]
-             thread_set_ipc_tcb_cap_valid
-             cap_delete_pas_refined'[THEN valid_validE_E] thread_set_cte_wp_at_trivial
-        | simp add: ran_tcb_cap_cases dom_tcb_cap_cases[simplified]
-                    emptyable_def a_type_def partial_inv_def
-               del: hoare_True_E_R
-        | wpc
-        | strengthen invs_mdb use_no_cap_to_obj_asid_strg
-                     tcb_cap_always_valid_strg[where p="tcb_cnode_index 0"]
-                     tcb_cap_always_valid_strg[where p="tcb_cnode_index (Suc 0)"]
-        )+
-  apply (clarsimp simp: authorised_tcb_inv_def)
-  apply (clarsimp simp: tcb_at_cte_at_0 tcb_at_cte_at_1[simplified]
-                        is_cap_simps is_valid_vtable_root_def
-                        is_cnode_or_valid_arch_def tcb_cap_valid_def
-                        tcb_at_st_tcb_at[symmetric] invs_valid_objs
-                        cap_asid_def vs_cap_ref_def
-                        clas_no_asid cli_no_irqs
-                        emptyable_def
-       | rule conjI | erule pas_refined_refl)+
-  done
-
 lemma invoke_tcb_unbind_notification_respects:
-  "\<lbrace>integrity aag X st and pas_refined aag and simple_sched_action
-       and einvs and Tcb_AI.tcb_inv_wf (tcb_invocation.NotificationControl t None)
-       and K (authorised_tcb_inv aag (tcb_invocation.NotificationControl t None))\<rbrace>
-     invoke_tcb (tcb_invocation.NotificationControl t None)
-   \<lbrace>\<lambda>rv. integrity aag X st\<rbrace>"
+  "\<lbrace>integrity aag X st and pas_refined aag and simple_sched_action and einvs
+                       and tcb_inv_wf (NotificationControl t None)
+                       and K (authorised_tcb_inv aag (NotificationControl t None))\<rbrace>
+   invoke_tcb (tcb_invocation.NotificationControl t None)
+   \<lbrace>\<lambda>_. integrity aag X st\<rbrace>"
   apply (clarsimp)
   apply (wp unbind_notification_respects)
   apply (clarsimp simp: authorised_tcb_inv_def tcb_at_def pred_tcb_def2)
@@ -362,10 +239,10 @@ lemma invoke_tcb_unbind_notification_respects:
   done
 
 lemma sbn_bind_respects:
-  "\<lbrace>integrity aag X st and bound_tcb_at ((=) None) t
-    and K ((pasSubject aag, Receive, pasObjectAbs aag ntfn) \<in> pasPolicy aag \<and> is_subject aag t)\<rbrace>
-       set_bound_notification t (Some ntfn)
-   \<lbrace>\<lambda>rv. integrity aag X st \<rbrace>"
+  "\<lbrace>integrity aag X st and bound_tcb_at ((=) None) t and
+    K (aag_has_auth_to aag Receive ntfn \<and> is_subject aag t)\<rbrace>
+   set_bound_notification t (Some ntfn)
+   \<lbrace>\<lambda>_. integrity aag X st \<rbrace>"
   apply (simp add: set_bound_notification_def)
   apply (wpsimp wp: set_object_wp)
   apply (erule integrity_trans)
@@ -375,10 +252,9 @@ lemma sbn_bind_respects:
 
 lemma bind_notification_respects:
   "\<lbrace>integrity aag X st and pas_refined aag and bound_tcb_at ((=) None) t
-      and K ((pasSubject aag, Receive, pasObjectAbs aag ntfnptr) \<in> pasPolicy aag \<and>
-             is_subject aag t)\<rbrace>
-     bind_notification t ntfnptr
-   \<lbrace>\<lambda>rv. integrity aag X st\<rbrace>"
+                       and K (aag_has_auth_to aag Receive ntfn \<and> is_subject aag t)\<rbrace>
+   bind_notification t ntfn
+   \<lbrace>\<lambda>_. integrity aag X st\<rbrace>"
   apply (rule hoare_gen_asm)
   apply (clarsimp simp: bind_notification_def)
   apply (rule hoare_seq_ext[OF _ get_simple_ko_sp])
@@ -387,12 +263,11 @@ lemma bind_notification_respects:
   done
 
 lemma invoke_tcb_bind_notification_respects:
-  "\<lbrace>integrity aag X st and pas_refined aag
-      and einvs and Tcb_AI.tcb_inv_wf (tcb_invocation.NotificationControl t (Some ntfn))
-      and simple_sched_action
-      and K (authorised_tcb_inv aag (tcb_invocation.NotificationControl t (Some ntfn)))\<rbrace>
-     invoke_tcb (tcb_invocation.NotificationControl t (Some ntfn))
-   \<lbrace>\<lambda>rv. integrity aag X st\<rbrace>"
+  "\<lbrace>integrity aag X st and pas_refined aag and einvs and simple_sched_action
+                       and tcb_inv_wf (NotificationControl t (Some ntfn))
+                       and K (authorised_tcb_inv aag (NotificationControl t (Some ntfn)))\<rbrace>
+   invoke_tcb (NotificationControl t (Some ntfn))
+   \<lbrace>\<lambda>_. integrity aag X st\<rbrace>"
   apply (rule hoare_gen_asm)
   apply (clarsimp)
   apply (wp bind_notification_respects)
@@ -400,71 +275,90 @@ lemma invoke_tcb_bind_notification_respects:
   done
 
 lemma invoke_tcb_ntfn_control_respects[wp]:
-  "\<lbrace>integrity aag X st and pas_refined aag
-      and einvs and Tcb_AI.tcb_inv_wf (tcb_invocation.NotificationControl t ntfn)
-      and simple_sched_action
-      and K (authorised_tcb_inv aag (tcb_invocation.NotificationControl t ntfn))\<rbrace>
-     invoke_tcb (tcb_invocation.NotificationControl t ntfn)
-   \<lbrace>\<lambda>rv. integrity aag X st\<rbrace>"
+  "\<lbrace>integrity aag X st and pas_refined aag and einvs and simple_sched_action
+                       and tcb_inv_wf (NotificationControl t ntfn)
+                       and K (authorised_tcb_inv aag (NotificationControl t ntfn))\<rbrace>
+   invoke_tcb (NotificationControl t ntfn)
+   \<lbrace>\<lambda>_. integrity aag X st\<rbrace>"
   apply (case_tac ntfn, simp_all del: invoke_tcb.simps Tcb_AI.tcb_inv_wf.simps K_def)
    apply (wp invoke_tcb_bind_notification_respects invoke_tcb_unbind_notification_respects | simp)+
   done
 
+
+locale Tcb_AC_1 =
+  fixes aag :: "'a PAS"
+  assumes arch_post_modify_registers_invs[wp]:
+    "arch_post_modify_registers cur t \<lbrace>pas_refined aag\<rbrace>"
+  and arch_post_modify_registers_respects:
+    "\<lbrace>integrity aag X st and K (is_subject aag t)\<rbrace>
+     arch_post_modify_registers cur t
+     \<lbrace>\<lambda>_ s. integrity aag X st s\<rbrace>"
+  and arch_get_sanitise_register_info_inv[wp]:
+    "arch_get_sanitise_register_info t \<lbrace>\<lambda>s :: det_ext state. P s\<rbrace>"
+  and invoke_tcb_tc_respects_aag:
+    "\<lbrace>integrity aag X st and pas_refined aag and einvs and simple_sched_action
+                         and tcb_inv_wf (ThreadControl t sl ep mcp priority croot vroot buf)
+                         and K (authorised_tcb_inv aag (ThreadControl t sl ep mcp priority croot vroot buf))\<rbrace>
+     invoke_tcb (ThreadControl t sl ep mcp priority croot vroot buf)
+     \<lbrace>\<lambda>rv. integrity aag X st and pas_refined aag\<rbrace>"
+begin
+
 lemma invoke_tcb_respects:
-  "\<lbrace>integrity aag X st and pas_refined aag
-         and einvs and simple_sched_action and Tcb_AI.tcb_inv_wf ti
-         and K (authorised_tcb_inv aag ti)\<rbrace>
-     invoke_tcb ti
-   \<lbrace>\<lambda>rv. integrity aag X st\<rbrace>"
+  "\<lbrace>integrity aag X st and pas_refined aag and einvs and simple_sched_action
+                       and tcb_inv_wf ti and K (authorised_tcb_inv aag ti)\<rbrace>
+   invoke_tcb ti
+   \<lbrace>\<lambda>_. integrity aag X st\<rbrace>"
   apply (cases ti, simp_all add: hoare_conjD1 [OF invoke_tcb_tc_respects_aag [simplified simp_thms]]
                             del: invoke_tcb.simps Tcb_AI.tcb_inv_wf.simps K_def)
   apply (safe intro!: hoare_gen_asm)
-  apply ((wp itr_wps mapM_x_wp' | simp add: if_apply_def2 split del: if_split
-            | wpc | clarsimp simp: authorised_tcb_inv_def arch_get_sanitise_register_info_def
-            | rule conjI | subst(asm) idle_no_ex_cap)+)
-  done
+  by ((wp itr_wps mapM_x_wp' arch_post_modify_registers_respects
+       | wpc | clarsimp simp: authorised_tcb_inv_def if_apply_def2
+       | rule conjI | subst (asm) idle_no_ex_cap)+)
+
+end
+
 
 subsubsection\<open>@{term "pas_refined"}\<close>
 
 lemmas ita_wps = as_user_pas_refined restart_pas_refined cap_insert_pas_refined
                  thread_set_pas_refined cap_delete_pas_refined' check_cap_inv2 hoare_vcg_all_liftE
-                 hoare_weak_lift_impE hoare_weak_lift_imp hoare_vcg_all_lift
+                 wp_throw_const_impE hoare_weak_lift_imp hoare_vcg_all_lift
 
 lemma hoare_st_refl:
-  "\<lbrakk>\<And>st. \<lbrace>P st\<rbrace> f \<lbrace>Q st\<rbrace>; \<And>r s st. Q st r s \<Longrightarrow> Q' r s\<rbrakk> \<Longrightarrow> \<lbrace>\<lambda>s. P s s\<rbrace> f \<lbrace>Q'\<rbrace>"
+  "\<lbrakk> \<And>st. \<lbrace>P st\<rbrace> f \<lbrace>Q st\<rbrace>; \<And>r s st. Q st r s \<Longrightarrow> Q' r s \<rbrakk> \<Longrightarrow> \<lbrace>\<lambda>s. P s s\<rbrace> f \<lbrace>Q'\<rbrace>"
   apply (clarsimp simp add: valid_def)
   apply (drule_tac x=s in meta_spec)
   apply force
   done
 
 lemma bind_notification_pas_refined[wp]:
-  "\<lbrace>pas_refined aag
-      and K (\<forall>auth \<in> {Receive, Reset}.
-                   (pasObjectAbs aag t, auth, pasObjectAbs aag ntfnptr) \<in> pasPolicy aag)\<rbrace>
-     bind_notification t ntfnptr
+  "\<lbrace>pas_refined aag and K (\<forall>auth \<in> {Receive, Reset}. abs_has_auth_to aag auth t ntfn)\<rbrace>
+   bind_notification t ntfn
    \<lbrace>\<lambda>_. pas_refined aag\<rbrace>"
   apply (clarsimp simp: bind_notification_def)
   apply (wp set_simple_ko_pas_refined | wpc | simp)+
   done
 
 lemma invoke_tcb_ntfn_control_pas_refined[wp]:
-  "\<lbrace>pas_refined aag and Tcb_AI.tcb_inv_wf (tcb_invocation.NotificationControl t ntfn)
-     and einvs  and simple_sched_action
-     and K (authorised_tcb_inv aag (tcb_invocation.NotificationControl t ntfn))\<rbrace>
-     invoke_tcb (tcb_invocation.NotificationControl t ntfn)
+  "\<lbrace>pas_refined aag and tcb_inv_wf (NotificationControl t ntfn) and einvs and simple_sched_action
+                    and K (authorised_tcb_inv aag (NotificationControl t ntfn))\<rbrace>
+   invoke_tcb (NotificationControl t ntfn)
    \<lbrace>\<lambda>_. pas_refined aag\<rbrace>"
   apply (case_tac ntfn, simp_all del: K_def)
    apply (safe intro!: hoare_gen_asm)
    apply (wp | simp add: authorised_tcb_inv_def)+
   done
 
+
+context Tcb_AC_1 begin
+
 lemma invoke_tcb_pas_refined:
-  "\<lbrace>pas_refined aag and Tcb_AI.tcb_inv_wf ti and einvs and simple_sched_action
-       and K (authorised_tcb_inv aag ti)\<rbrace>
-     invoke_tcb ti
-   \<lbrace>\<lambda>rv. pas_refined aag\<rbrace>"
+  "\<lbrace>pas_refined aag and tcb_inv_wf ti and einvs and simple_sched_action
+                    and K (authorised_tcb_inv aag ti)\<rbrace>
+   invoke_tcb ti
+   \<lbrace>\<lambda>_. pas_refined aag\<rbrace>"
   apply (cases "\<exists>t sl ep mcp priority croot vroot buf.
-              ti = tcb_invocation.ThreadControl t sl ep mcp priority croot vroot buf")
+                ti = tcb_invocation.ThreadControl t sl ep mcp priority croot vroot buf")
    apply safe
    apply (rule hoare_chain, rule_tac Q'="\<lambda>_. pas_refined aag" and st1="\<lambda>x. x" in
                                      hoare_st_refl[OF invoke_tcb_tc_respects_aag])
@@ -475,72 +369,77 @@ lemma invoke_tcb_pas_refined:
   apply (cases ti, simp_all add: authorised_tcb_inv_def)
         apply (wp ita_wps hoare_drop_imps mapM_x_wp'
               | simp add: emptyable_def if_apply_def2 authorised_tcb_inv_def
-                          arch_get_sanitise_register_info_def
               | rule ball_tcb_cap_casesI
               | wpc
               | fastforce intro: notE[rotated,OF idle_no_ex_cap,simplified]
                            simp: invs_valid_global_refs invs_valid_objs)+
   done
 
+end
+
+
 subsection\<open>TCB / decode\<close>
 
 lemma decode_registers_authorised:
-  "\<lbrace>K (is_subject aag t)\<rbrace> decode_read_registers msg (cap.ThreadCap t) \<lbrace>\<lambda>rv s. authorised_tcb_inv aag rv\<rbrace>, -"
-  "\<lbrace>K (is_subject aag t)\<rbrace> decode_write_registers msg (cap.ThreadCap t) \<lbrace>\<lambda>rv s. authorised_tcb_inv aag rv\<rbrace>, -"
-  "\<lbrace>pas_refined aag and K (is_subject aag t \<and> (\<forall>(cap, slot) \<in> set excaps. pas_cap_cur_auth aag cap \<and> is_subject aag (fst slot)))\<rbrace>
-     decode_copy_registers msg (cap.ThreadCap t) (map fst excaps)
-   \<lbrace>\<lambda>rv s. authorised_tcb_inv aag rv\<rbrace>, -"
-  unfolding decode_read_registers_def decode_write_registers_def decode_copy_registers_def authorised_tcb_inv_def
-  by (rule hoare_pre, simp cong: list.case_cong, (wp | wpc)+, clarsimp simp: cap_auth_conferred_def pas_refined_all_auth_is_owns aag_cap_auth_def)+
-
-
-lemma stupid_strg:
-  "cap_links_asid_slot aag (pasObjectAbs aag (fst y)) x \<longrightarrow>
-  (x = cap \<and> (\<exists>b. y = (a, b)) \<longrightarrow> cap_links_asid_slot aag (pasObjectAbs aag a) cap)"
-  by auto
+  "\<lbrace>K (is_subject aag t)\<rbrace> decode_read_registers msg (ThreadCap t) \<lbrace>\<lambda>rv s. authorised_tcb_inv aag rv\<rbrace>, -"
+  "\<lbrace>K (is_subject aag t)\<rbrace> decode_write_registers msg (ThreadCap t) \<lbrace>\<lambda>rv s. authorised_tcb_inv aag rv\<rbrace>, -"
+  "\<lbrace>pas_refined aag and K (is_subject aag t \<and> (\<forall>(cap, slot) \<in> set excaps. pas_cap_cur_auth aag cap
+                                                                        \<and> is_subject aag (fst slot)))\<rbrace>
+   decode_copy_registers msg (ThreadCap t) (map fst excaps)
+   \<lbrace>\<lambda>rv _. authorised_tcb_inv aag rv\<rbrace>, -"
+  unfolding decode_read_registers_def decode_write_registers_def
+            decode_copy_registers_def authorised_tcb_inv_def
+    apply (simp_all cong: list.case_cong)
+    apply wpsimp+
+  apply (clarsimp simp: cap_auth_conferred_def pas_refined_all_auth_is_owns aag_cap_auth_def)
+  done
 
 lemma decode_set_ipc_buffer_authorised:
   "\<lbrace>K (is_subject aag t \<and> (\<forall>x \<in> set excaps. is_subject aag (fst (snd x)))
-                      \<and> (\<forall>x \<in> set excaps. pas_cap_cur_auth aag (fst x))) \<rbrace>
-    decode_set_ipc_buffer msg (cap.ThreadCap t) slot excaps
-   \<lbrace>\<lambda>rv s. authorised_tcb_inv aag rv\<rbrace>, -"
+                        \<and> (\<forall>x \<in> set excaps. pas_cap_cur_auth aag (fst x)))\<rbrace>
+   decode_set_ipc_buffer msg (ThreadCap t) slot excaps
+   \<lbrace>\<lambda>rv _ :: det_ext state. authorised_tcb_inv aag rv\<rbrace>, -"
   unfolding decode_set_ipc_buffer_def authorised_tcb_inv_def
   apply (cases "excaps ! 0")
   apply (clarsimp cong: list.case_cong split del: if_split)
   apply (rule hoare_pre)
   apply (clarsimp simp: ball_Un aag_cap_auth_def split del: if_split split: prod.split
-       | strengthen stupid_strg
-       | wp (once) derive_cap_obj_refs_auth derive_cap_untyped_range_subset derive_cap_clas derive_cap_cli
-                 hoare_vcg_all_lift_R whenE_throwError_wp slot_long_running_inv
-       | wpc)+
+         | wp (once) derive_cap_obj_refs_auth derive_cap_untyped_range_subset derive_cap_clas
+                     derive_cap_cli hoare_vcg_all_lift_R whenE_throwError_wp slot_long_running_inv
+         | wpc)+
   apply (cases excaps, simp)
   apply fastforce
   done
 
 lemma decode_set_space_authorised:
   "\<lbrace>K (is_subject aag t \<and> (\<forall>x \<in> set excaps. is_subject aag (fst (snd x)))
-                      \<and> (\<forall>x \<in> set excaps. pas_cap_cur_auth aag (fst x))) \<rbrace>
-     decode_set_space ws (cap.ThreadCap t) slot excaps
-   \<lbrace>\<lambda>rv s. authorised_tcb_inv aag rv\<rbrace>, -"
+                        \<and> (\<forall>x \<in> set excaps. pas_cap_cur_auth aag (fst x)))\<rbrace>
+   decode_set_space ws (ThreadCap t) slot excaps
+   \<lbrace>\<lambda>rv _ :: det_ext state. authorised_tcb_inv aag rv\<rbrace>, -"
   unfolding decode_set_space_def authorised_tcb_inv_def
   apply (rule hoare_pre)
   apply (simp cong: list.case_cong split del: if_split)
   apply (clarsimp simp: ball_Un split del: if_split
-       | wp (once) derive_cap_obj_refs_auth derive_cap_untyped_range_subset derive_cap_clas derive_cap_cli
-                 hoare_vcg_const_imp_lift_R hoare_vcg_all_lift_R whenE_throwError_wp slot_long_running_inv)+
+         | wp (once) derive_cap_obj_refs_auth derive_cap_untyped_range_subset derive_cap_clas
+                     derive_cap_cli hoare_vcg_const_imp_lift_R hoare_vcg_all_lift_R
+                     whenE_throwError_wp slot_long_running_inv)+
   apply (clarsimp simp: not_less all_set_conv_all_nth dest!: P_0_1_spec)
-  apply (auto simp: aag_cap_auth_def update_cap_cli intro: update_cap_obj_refs_subset dest!: update_cap_untyped_range_subset update_cap_cap_auth_conferred_subset)
+  apply (auto simp: aag_cap_auth_def update_cap_cli
+             intro: update_cap_obj_refs_subset
+             dest!: update_cap_cap_auth_conferred_subset)
   done
 
 (* grot: this is from the bowels of decode_tcb_configure_authorised. *)
 lemma decode_tcb_configure_authorised_helper:
   "\<lbrace>K True and K (is_subject aag t \<and> (\<forall>x \<in> set excaps. is_subject aag (fst (snd x)))
-                      \<and> (\<forall>x \<in> set excaps. pas_cap_cur_auth aag (fst x))
-                      \<and> authorised_tcb_inv aag set_param \<and> is_thread_control set_param)\<rbrace>
-     decode_set_space ws (cap.ThreadCap t) slot excaps
-   \<lbrace>\<lambda>rv s. authorised_tcb_inv aag (tcb_invocation.ThreadControl t slot (tc_new_fault_ep rv)
-                                    None None (tc_new_croot rv)
-                                    (tc_new_vroot rv) (tc_new_buffer set_param))\<rbrace>, -"
+                                   \<and> (\<forall>x \<in> set excaps. pas_cap_cur_auth aag (fst x))
+                                   \<and> authorised_tcb_inv aag set_param
+                                   \<and> is_thread_control set_param)\<rbrace>
+   decode_set_space ws (ThreadCap t) slot excaps
+   \<lbrace>\<lambda>rv _ :: det_ext state. authorised_tcb_inv aag (ThreadControl t slot (tc_new_fault_ep rv)
+                                                                  None None (tc_new_croot rv)
+                                                                  (tc_new_vroot rv)
+                                                                  (tc_new_buffer set_param))\<rbrace>, -"
   apply (rule hoare_gen_asmE)
   apply (cases set_param)
   apply (simp_all add: is_thread_control_def decode_set_space_def authorised_tcb_inv_def
@@ -550,19 +449,20 @@ lemma decode_tcb_configure_authorised_helper:
   apply (cases "excaps!Suc 0")
   apply (rule hoare_pre)
    apply (clarsimp simp: ball_Un split del: if_split split: prod.split
-        | strengthen stupid_strg
         | wp (once) derive_cap_obj_refs_auth derive_cap_untyped_range_subset derive_cap_clas derive_cap_cli
                   hoare_vcg_all_lift_R whenE_throwError_wp slot_long_running_inv)+
   apply (clarsimp cong: list.case_cong option.case_cong prod.case_cong split: prod.split_asm)
   apply (clarsimp simp: not_less all_set_conv_all_nth dest!: P_0_1_spec)
-  apply (auto simp: aag_cap_auth_def update_cap_cli intro: update_cap_untyped_range_subset update_cap_obj_refs_subset dest!: update_cap_cap_auth_conferred_subset elim: bspec)
+  apply (auto simp: aag_cap_auth_def update_cap_cli
+             intro: update_cap_obj_refs_subset
+             dest!: update_cap_cap_auth_conferred_subset)
   done
 
 lemma decode_tcb_configure_authorised:
   "\<lbrace>K (is_subject aag t \<and> (\<forall>x \<in> set excaps. is_subject aag (fst (snd x)))
-                      \<and> (\<forall>x \<in> set excaps. pas_cap_cur_auth aag (fst x))) \<rbrace>
-    decode_tcb_configure msg (cap.ThreadCap t) slot excaps
-   \<lbrace>\<lambda>rv s. authorised_tcb_inv aag rv\<rbrace>, -"
+                        \<and> (\<forall>x \<in> set excaps. pas_cap_cur_auth aag (fst x)))\<rbrace>
+   decode_tcb_configure msg (ThreadCap t) slot excaps
+   \<lbrace>\<lambda>rv _ :: det_ext state. authorised_tcb_inv aag rv\<rbrace>, -"
   apply (wpsimp simp: decode_tcb_configure_def
                 wp: whenE_throwError_wp decode_tcb_configure_authorised_helper
                     decode_set_ipc_buffer_authorised)
@@ -571,26 +471,26 @@ lemma decode_tcb_configure_authorised:
 
 lemma decode_set_priority_authorised:
   "\<lbrace>K (is_subject aag t)\<rbrace>
-    decode_set_priority msg (ThreadCap t) slot excs
-   \<lbrace>\<lambda>rv s. authorised_tcb_inv aag rv\<rbrace>, -"
+   decode_set_priority msg (ThreadCap t) slot excs
+   \<lbrace>\<lambda>rv _. authorised_tcb_inv aag rv\<rbrace>, -"
   by (wpsimp simp: decode_set_priority_def check_prio_def authorised_tcb_inv_def)
 
 lemma decode_set_mcpriority_authorised:
   "\<lbrace>K (is_subject aag t)\<rbrace>
-    decode_set_mcpriority msg (ThreadCap t) slot excs
-   \<lbrace>\<lambda>rv s. authorised_tcb_inv aag rv\<rbrace>, -"
+   decode_set_mcpriority msg (ThreadCap t) slot excs
+   \<lbrace>\<lambda>rv _. authorised_tcb_inv aag rv\<rbrace>, -"
   by (wpsimp simp: decode_set_mcpriority_def check_prio_def authorised_tcb_inv_def)
 
 lemma decode_set_sched_params_authorised:
   "\<lbrace>K (is_subject aag t)\<rbrace>
-    decode_set_sched_params msg (ThreadCap t) slot excs
-   \<lbrace>\<lambda>rv s. authorised_tcb_inv aag rv\<rbrace>, -"
+   decode_set_sched_params msg (ThreadCap t) slot excs
+   \<lbrace>\<lambda>rv _. authorised_tcb_inv aag rv\<rbrace>, -"
   by (wpsimp simp: decode_set_sched_params_def check_prio_def authorised_tcb_inv_def)
 
 lemma decode_unbind_notification_authorised:
   "\<lbrace>K (is_subject aag t)\<rbrace>
-    decode_unbind_notification (cap.ThreadCap t)
-   \<lbrace>\<lambda>rv s. authorised_tcb_inv aag rv\<rbrace>, -"
+   decode_unbind_notification (ThreadCap t)
+   \<lbrace>\<lambda>rv _. authorised_tcb_inv aag rv\<rbrace>, -"
   unfolding decode_unbind_notification_def authorised_tcb_inv_def
   apply clarsimp
   apply (wp gbn_wp, clarsimp)
@@ -598,9 +498,9 @@ lemma decode_unbind_notification_authorised:
 
 lemma decode_bind_notification_authorised:
   "\<lbrace>K (is_subject aag t \<and> (\<forall>x \<in> set excaps. is_subject aag (fst (snd x)))
-                      \<and> (\<forall>x \<in> set excaps. pas_cap_cur_auth aag (fst x)) )\<rbrace>
-    decode_bind_notification (cap.ThreadCap t) excaps
-   \<lbrace>\<lambda>rv s. authorised_tcb_inv aag rv\<rbrace>, -"
+                        \<and> (\<forall>x \<in> set excaps. pas_cap_cur_auth aag (fst x)) )\<rbrace>
+   decode_bind_notification (ThreadCap t) excaps
+   \<lbrace>\<lambda>rv _. authorised_tcb_inv aag rv\<rbrace>, -"
   unfolding decode_bind_notification_def authorised_tcb_inv_def
   apply clarsimp
   apply (wp gbn_wp get_simple_ko_wp whenE_throwError_wp | wpc | simp add:)+
@@ -611,18 +511,19 @@ lemma decode_bind_notification_authorised:
 
 lemma decode_set_tls_base_authorised:
   "\<lbrace>K (is_subject aag t)\<rbrace>
-    decode_set_tls_base msg (cap.ThreadCap t)
-   \<lbrace>\<lambda>rv s. authorised_tcb_inv aag rv\<rbrace>, -"
+   decode_set_tls_base msg (ThreadCap t)
+   \<lbrace>\<lambda>rv _. authorised_tcb_inv aag rv\<rbrace>, -"
   unfolding decode_set_tls_base_def authorised_tcb_inv_def
   apply clarsimp
   apply (wpsimp wp: gbn_wp)
   done
 
 lemma decode_tcb_invocation_authorised:
-  "\<lbrace>invs and pas_refined aag and K (is_subject aag t \<and> (\<forall>x \<in> set excaps. is_subject aag (fst (snd x)))
-                                  \<and> (\<forall>x \<in> set excaps. pas_cap_cur_auth aag (fst x)))\<rbrace>
-     decode_tcb_invocation label msg (cap.ThreadCap t) slot excaps
-   \<lbrace>\<lambda>rv s. authorised_tcb_inv aag rv\<rbrace>,-"
+  "\<lbrace>invs and pas_refined aag
+         and K (is_subject aag t \<and> (\<forall>x \<in> set excaps. is_subject aag (fst (snd x)))
+                                 \<and> (\<forall>x \<in> set excaps. pas_cap_cur_auth aag (fst x)))\<rbrace>
+   decode_tcb_invocation label msg (ThreadCap t) slot excaps
+   \<lbrace>\<lambda>rv _. authorised_tcb_inv aag rv\<rbrace>, -"
   unfolding decode_tcb_invocation_def
   apply (rule hoare_pre)
    apply wpc
@@ -641,7 +542,5 @@ text\<open>
 to show @{term "integrity"} or @{term "pas_refined"}.
 
 \<close>
-
-end
 
 end
